iodiv/Tests2.fst
@@ -1,0 +1,119 @@
+module Tests2
+
+open FStar.List.Tot
+open FStar.List.Tot.Properties
+open FStar.Tactics // Also defines forall_intro so place before Classical
+open FStar.Classical
+open FStar.IndefiniteDescription
+open FStar.Calc
+open FStar.FunctionalExtensionality
+open Util
+open Stream
+open Itree
+open IODivHist
+
+unfold
+let ret_trace #a (r : branch a) : Pure trace (requires terminates r) (ensures fun _ -> True) =
+  match r with
+  | Fin tr x -> tr
+
+unfold
+let result #a (r : branch a) : Pure a (requires terminates r) (ensures fun _ -> True) =
+  match r with
+  | Fin tr x -> x
+
+let act_call (o : cmds) (x : io_args o) : IODiv (io_res o) (requires fun hist -> forall y. valid_event hist (choice_to_event (Call_choice o x y))) (ensures fun hist r -> terminates r /\ ret_trace r == [ choice_to_event (Call_choice o x (result r)) ]) =
+  IODIV?.reflect (iodiv_call _ o x (fun y -> iodiv_ret _ y))
+
+let open_file (s : string) : IODiv file_descr (requires fun hist -> True) (ensures fun hist r -> terminates r /\ ret_trace r == [ EOpenfile s (result r) ]) =
+  act_call Openfile s
+
+let read (fd : file_descr) : IODiv string (requires fun hist -> is_open hist fd) (ensures fun hist r -> terminates r /\ ret_trace r == [ ERead fd (result r) ]) =
+  act_call Read fd
+
+let close (fd : file_descr) : IODiv unit (requires fun hist -> is_open hist fd) (ensures fun hist r -> terminates r /\ ret_trace r == [ EClose fd (result r) ]) =
+  act_call Close fd
+
+// let repeat_inv #w (body : unit -> IODIV unit w) (inv : (trace -> Type0) { trace_invariant w inv }) : IODIV unit (pwrepeat_inv w inv) =
+//   IODIV?.reflect (piodiv_repeat_with_inv (reify (body ())) inv)
+
+assume val get_trace : unit -> IODiv trace (fun hist -> True) (ensures fun hist r -> terminates r /\ result r == hist)
+
+let test_1 (s : string) : IODiv string (requires fun h -> True) (ensures fun _ _ -> True)
+by (
+  explode () ;
+  bump_nth 2 ;
+  branch_on_match () ;
+  explode () ;
+  unfold_def (`is_open) ;
+  norm [ iota ] ;
+  dump "h"
+)
+=
+  let fd = open_file s in
+  read fd
+
+let test_1' (s : string) : IODiv string (requires True) (ensures fun _ -> True)
+= let fd = open_file s in
+  let fd' = open_file s in
+  read fd
+
+let test_2 (s : string) : IODiv file_descr (requires True) (ensures fun _ -> True) =
+  let msg = test_1 s in
+  open_file s
+
+let test (s : string) : IODiv unit (requires True) (ensures fun _ -> True) =
+  let fd = open_file s in
+  let msg = read fd in
+  close fd
+
+let test_ (s : string) : IODiv unit (requires True) (ensures fun r -> terminates r /\ (exists fd msg. ret_trace r == [ EOpenfile s fd ; ERead fd msg ; EClose fd () ]))
+= let fd = open_file s in
+  let msg = read fd in
+  close fd
+
+let test'' (fd : file_descr) : IODiv unit (requires True) (ensures fun _ -> True) =
+  let msg = read fd in
+  ()
+
+let test_more (fd : file_descr) : IODiv unit (requires True) (ensures fun _ -> True) =
+  test'' fd ; test'' fd
+
+let test_more' (fd : file_descr) : IODiv unit (requires True) (ensures fun _ -> True) =
+  test'' fd ;
+  test'' fd ;
+  test'' fd
+
+let test3 (fd : file_descr) : IODiv unit (requires True) (ensures fun _ -> True) =
+  let msg = read fd in
+  () ; () ; ()
+
+let test' (s : string) : IODiv unit (requires True) (ensures fun _ -> True)
+= let fd = open_file s in
+  let msg = read fd in
+  ()
+
+let test'_ (s : string) : IODiv string (requires True) (ensures fun _ -> True) =
+  let fd = open_file s in
+  read fd
+
+let open_close_test (s : string) : IODiv unit (requires True) (ensures fun r -> terminates r /\ (exists fd. ret_trace r == [ EOpenfile s fd ; EClose fd () ])) =
+  let fd = open_file s in
+  close fd
+
+let many_open_test (s : string) : IODiv unit (requires True) (ensures fun r -> terminates r)
+= let x = open_file s in
+  let y = open_file s in
+  ()
+
+let many_open_test' (s : string) : IODiv file_descr (requires True) (ensures fun r -> terminates r) =
+  let x = open_file s in
+  open_file s
+
+// Fails because it can't infer something (the w??)
+// let repeat_open_close_test (s : string) : IODiv unit (requires True) (ensures fun _ -> True) =
+//   repeat_inv (fun _ -> open_close_test s) (fun _ -> True)
+
+// Similar problem it seems
+// let repeat_pure (t : unit -> unit) : IODiv unit (requires True) (ensures fun r -> True) =
+//   repeat_inv t (fun _ -> True)
